Test/VProg.v
@@ -1,14 +1,11 @@
 Require Import SLFun.Util SLFun.Values SLFun.SL.
 Require Import SLFun.VProg.
-Require SLFun.ConcreteProg SLFun.SLProg.
 
 Require Import Coq.Lists.List.
 
-Module CP := SLFun.ConcreteProg.
-Module SP := SLFun.SLProg.
-
 Import SLNotations.
 Import ListNotations.
+Import VProg._Abbrev.
 
 
 Definition f_main : fid := 0.
@@ -53,14 +50,6 @@ Proof.
   eexists. reflexivity.
 Defined.
 
-Lemma reduce_spec_t [A ctx] [P : i_spec_t A ctx -> Prop] [s0 s1]
-  (H : P s0)
-  (E : s0 = s1):
-  P s1.
-Proof.
-  rewrite <- E; exact H.
-Qed.
-
 Lemma sls_main (ps : ptr * ptr):
   SP.sls SPEC (proj1_sig (impl_main ps)) (spec_main_n ps).
 Proof.
@@ -72,51 +61,37 @@ Proof.
   eapply SP.Cons.
   - eapply (proj2_sig (i_spec (vprog_main _) [CTX.mka (SLprop.cell p0, v0); CTX.mka (SLprop.cell p1, v1)]))
       with (post := fun _ => True).
-    + eapply reduce_spec_t. hnf.
-      unshelve refine (@Bind_SpecI _ _ _ _ _ _ _ _ _ _ _ _ _). 3,4:shelve.
-      1:eexists. 2-5:cbn.
-      { eapply reduce_spec_t. hnf.
-        unshelve refine (@Read_SpecI _ _ _ _). 1:shelve.
-        unshelve eexists. 3:cbn.
+    + simple refine (Bind_SpecI1 _ _ _ _ _ _ _ _ _ _). 1,3,5,7,9,11,13:shelve.
+      { hnf.
+        simple refine (@Read_SpecI _ _ _ _). 1:shelve.
+        unshelve eexists.
         - exact (Vector.cons _ true _ (Vector.cons _ false _ (Vector.nil _))).
-        - cbn; SLprop.normalize; reflexivity.
-        - cbn; reflexivity. }
-
-      cbn.
-      epose (spec_0 := _).
-      intros x sls_0; unshelve eexists; case sls_0 as [].
-      exact (spec_0 x). unfold spec_0; clear spec_0. 2-4:cbn.
-      eapply reduce_spec_t.
-      unshelve refine (@Bind_SpecI _ _ _ _ _ _ _ _ _ _ _ _ _). 3,4:shelve.
-      1:eexists. 2-5:cbn.
-      { eapply reduce_spec_t. hnf.
-        unshelve refine (@Write_SpecI _ _ _ _ _). 1:shelve.
-        unshelve eexists. 3:cbn.
+        - cbn; SLprop.normalize; reflexivity. }
+      { cbn; repeat intro. reflexivity. }
+      cbn; repeat intro.
+      simple refine (Bind_SpecI1 _ _ _ _ _ _ _ _ _ _). 1,3,5,7,9,11,13:shelve.
+      { unshelve refine (@Write_SpecI _ _ _ _ _). 1:shelve.
+        unshelve eexists.
         - exact (Vector.cons _ false _ (Vector.cons _ true _ (Vector.nil _))).
-        - cbn; SLprop.normalize; reflexivity.
-        - cbn; reflexivity. }
-
-      cbn.
-      epose (spec_1 := ?[spec_1]).
-      intros _u sls_1; unshelve eexists; case sls_1 as [sl_1 []].
-      exact (spec_1 _u sl_1). unfold spec_1; clear spec_1. 2-4:cbn.
-      { eapply reduce_spec_t.
-        unshelve refine (@Assert_SpecI _ _ _ _ _).
+        - cbn; SLprop.normalize; reflexivity. }
+      { cbn; repeat intro. reflexivity. }
+      cbn; repeat intro.
+      { unshelve refine (@Assert_SpecI _ _ _ _ _).
         1:repeat (constructor; [shelve|]); constructor.
-        all:cbn.
-        - unshelve eexists.
-          + exact (Vector.cons _ false _ (Vector.cons _ true _ (Vector.nil _))).
-          + cbn; SLprop.normalize; reflexivity.
-        - cbn; reflexivity. }
-
-      intros ? [? []]; cbn; reflexivity.
-      intros ? [? []]; cbn; reflexivity.
-      unfold _Abbrev.TF.arrow_ext, _Abbrev.TF.arrow_of_fun, sf_rsel; cbn. reflexivity.
-      intros ? []; cbn; reflexivity.
-      intros ? []; cbn; reflexivity.
-      unfold _Abbrev.TF.arrow_ext, _Abbrev.TF.arrow_of_fun, sf_rsel; cbn. reflexivity.
-    + cbn. auto.
-  - unfold sf_post, sf_post_ctx; cbn.
+        cbn.
+        unshelve eexists.
+        - exact (Vector.cons _ false _ (Vector.cons _ true _ (Vector.nil _))).
+        - cbn; SLprop.normalize; reflexivity. }
+      { cbn; repeat intro. reflexivity. }
+      { cbn; repeat intro. reflexivity. }
+      { cbn; repeat intro. reflexivity. }
+      { cbn; repeat intro. reflexivity. }
+      { cbn; repeat intro. reflexivity. }
+      { cbn; repeat intro. reflexivity. }
+      { cbn; repeat intro. reflexivity. }
+      { cbn; repeat intro. reflexivity. }
+    + unfold FP.BindA. cbn. auto.
+  - cbn.
     split; cbn.
     + SLprop.normalize. reflexivity.
     + constructor.
